Definition of up for interop

src/test/interop/Interop.fst
@@ -1,4 +1,5 @@
 module Interop
+
 (** Attempt to define down and up functions, to express relation between
     Low*'s and Vale's memory models.
     Currently only supports buffers of UInt8
@@ -31,6 +32,26 @@ let update_vale_mem mem buf heap =
       aux (i+1) (curr_heap.[addr + i] <- FStar.Seq.index contents i)
   in aux 0 heap
 
+(* Copy write_buffer from FStar.Pointer.Base, replacing Stack effect by Tot *)
+assume val write_buffer
+  (#t: P.typ)
+  (b: P.buffer t)
+  (i: UInt32.t)
+  (v: P.type_of_typ t)
+  (mem: HS.mem)
+  : HS.mem
+
+(* Takes a buffer, the previous HyperStack, and a low-level Vale Heap, and reconstructs the buffer
+   from the data in the Vale Heap *)
+val reconstruct_buf: P.(buffer (TBase TUInt8)) -> HS.mem -> Vale_Sem.heap -> GTot HS.mem
+let reconstruct_buf buf mem heap =
+  let addr = P.buffer_as_addr buf in
+  let length = P.buffer_length buf in
+  let rec aux (i:nat{i <= UInt32.v length}) curr_mem : GTot HS.mem (decreases %[sub length i]) =
+    if i >= (UInt32.v length) then curr_mem
+    else
+      aux (i+1) (write_buffer buf (UInt32.uint_to_t i) heap.[addr + i] curr_mem)
+  in aux 0 mem
 
 (* Takes a Low* Hyperstack, and a list of live buffers, and returns a low-level Vale heap
 containing these buffers *)
@@ -44,4 +65,13 @@ let down mem buffers =
   | [] -> accu_heap
   | a :: q -> aux q (update_vale_mem mem a accu_heap)
   in aux buffers heap
+  
+(* Takes a low-level Vale Heap and the initial Hyperstack, and reconstructs the buffers in the HyperStack *)
+val up: Vale_Sem.heap -> list P.(buffer (TBase TUInt8)) -> HS.mem -> GTot HS.mem
+
+let up heap buffers mem =
+  let rec aux bufs accu_mem heap : GTot HS.mem = match bufs with
+    | [] -> accu_mem
+    | a :: q -> aux q (reconstruct_buf a accu_mem heap) heap
+  in aux buffers mem heap
   
